new/proof/github_com/goose_lang/goose/testdata/examples/semantics_proof/slices.v
@@ -1,0 +1,16 @@
+From New.proof.github_com.goose_lang.goose.testdata.examples.semantics_proof
+       Require Import semantics_init.
+
+Section wps.
+Context `{!heapGS Σ}.
+Context {sem : go.Semantics} {package_sem : semantics.Assumptions}.
+Local Set Default Proof Using "All".
+
+Lemma wp_testSliceRef :
+  test_fun_ok semantics.testSliceRef.
+Proof.
+  semantics_auto.
+  (* TODO: translation bug for reference into slice *)
+Abort.
+
+End wps.
